

UC Berkeley CS285

homework 1: Imitation Learning

dhia naouali

November 7, 2025

1 Analysis

1. given

$$\frac{1}{T} \sum_{t=1}^T E_{p_{\pi^*}(s_t)} \pi_{\theta}(a_t \pi^*(s_t) | s_t) \leq \varepsilon$$
$$\sum_{t=1}^T E_{p_{\pi^*}(s_t)} \pi_{\theta}(a_t \pi^*(s_t) | s_t) \leq \varepsilon T$$

we introduce the event $M_t : \{\pi_{\theta}(a_t) \neq \pi^*(s_t)\}$
and by the union bound

$$\Pr\left(\bigcup_{k=1}^t M_k\right) \leq \sum_{k=1}^t \Pr(M_k) \leq \sum_{k=1}^T \Pr(M_k) \leq \varepsilon T$$

$$|p_{\pi_{\theta}}(s_t) - p_{\theta^*}(s_t)| = \Pr\left(\bigcup_t M_t\right) |p_{mistake}(s_t) - p_{\pi^*}(s_t)|$$

$$\sum_{s_t} |p_{\pi_{\theta}}(s_t) - p_{\theta^*}(s_t)| = \Pr\left(\bigcup_t M_t\right) \sum_{s_t} |p_{mistake}(s_t) - p_{\theta^*}(s_t)|$$

therefore

$$\sum_{s_t} |p_{\pi_{\theta}}(s_t) - p_{\theta^*}(s_t)| \leq 2\varepsilon T$$

2. (a) Given a state-dependent reward $r(s_t)$, where $|r(s_t)| \leq \mathcal{R}_{max}$, we consider the total expected reward:

$$\mathcal{J}(\pi) = \sum_{t=1}^T E_{p_{\pi^*}(s_t)} r(s_t)$$

$$\mathcal{J}(\pi^*) - \mathcal{J}(\pi_\theta) = \sum_{t=1}^T \left(E_{p_{\pi^*}(s_t)} r(s_t) - E_{p_{\pi_\theta}(s_t)} r(s_t) \right) = \sum_{t=1}^T E_{s_t} (p_{\pi^*}(s_t) - p_{\pi_\theta}(s_t)) r(s_t)$$

since $r(s_t) = 0$ for all $t < T$, we have:

$$\mathcal{J}(\pi^*) - \mathcal{J}(\pi_\theta) = \sum_{s_T} (p_{\pi^*}(s_T) - p_{\pi_\theta}(s_T)) \nabla(s_T).$$

thus,

$$\sum_{s_t} |p_{\pi^*}(s_t) - p_{\pi_\theta}(s_t)| \mathcal{R}_{\max} = \mathcal{O}(2\varepsilon T \mathcal{R}_{\max}) = \mathcal{O}(\varepsilon T).$$

(b) Given that

$$\mathcal{J}(\pi^*) - \mathcal{J}(\pi_\theta) = \sum_{t=1}^T \left(E_{p_{\pi^*}(s_t)} r(s_t) - E_{p_{\pi_\theta}(s_t)} r(s_t) \right),$$

where each term is $\mathcal{O}(2\varepsilon T \mathcal{R}_{\max})$, we get:

$$\mathcal{J}(\pi^*) - \mathcal{J}(\pi_\theta) = \mathcal{O}(2\varepsilon T^2 \mathcal{R}_{\max}) = \mathcal{O}(\varepsilon T^2).$$